coq/cilc2/clc_weakening.v
@@ -114,11 +114,387 @@ Proof with eauto 6 using merge, agree_ren.
     exists (_: G2)...
 Qed.
 
+Lemma arity_ren s A ξ : arity s A -> arity s A.[ren ξ].
+Proof with eauto using arity.
+  move=>ar. elim: ar ξ=>//={A}...
+  move=>A B ar ih ξ.
+  constructor.
+  asimpl.
+  apply: ih.
+Qed.
+
+Definition n_ren (ξ : var -> var) x :=
+  ξ x = x /\ forall i, (~x = i -> ~ξ i = x) /\ (~i = 0 -> ~ξ i = 0).
+
+Lemma n_ren0 ξ : n_ren (upren ξ) 0.
+Proof.
+  split; eauto.
+  move=> i. elim: i ξ=>//=.
+Qed.
+
+Lemma n_ren_up ξ x :
+  n_ren ξ x -> n_ren (upren ξ) x.+1.
+Proof.
+  move=>[e h]. split.
+  asimpl; eauto.
+  elim; asimpl; eauto.
+  move=>n [ih1 ih2]. split; eauto.
+  move=>neq.
+  have pf : ~x = n by eauto.
+  have[h1 h2]:=h n.
+  move: pf=>/h1; eauto.
+Qed.
+
+Lemma noccurs_ren x m ξ :
+  noccurs x m -> n_ren ξ x -> noccurs x m.[ren ξ].
+Proof with eauto using noccurs, n_ren_up, and.
+  move=>no. move: x m no ξ.
+  apply: noccurs_ind_nested...
+  move=>x y neq ξ [e h].
+  { have{h}[h _]:=h y.
+    move:neq=>/h neq.
+    constructor. eauto. }
+  move=>x A B s r t nA ihA nB ihB ξ n. asimpl.
+  { constructor. apply: ihA... apply: ihB... }
+  move=>x A m s t nA ihA nm ihm ξ n. asimpl.
+  { constructor. apply: ihA... apply: ihm... }
+  move=>x A Cs s nA ihA nCs ihCs ξ n. asimpl.
+  { constructor. apply: ihA...
+    elim: ihCs=>//=. constructor.
+    move=>m ls ihm _ ih.
+    constructor. asimpl...
+    asimpl in ih... }
+  move=>x m Q Fs nm ihm nQ ihQ nFs ihFs ξ. asimpl.
+  { constructor. apply: ihm... apply: ihQ...
+    elim: ihFs=>//=. constructor.
+    move=>m0 ls ihm0 _ ih.
+    constructor. asimpl...
+    asimpl in ih... }
+  move=>x A m nA ihA nm ihm ξ n. asimpl.
+  { constructor. apply: ihA... apply: ihm... }
+Qed.
+
+Lemma noccurs_ren_All1 x ms ξ :
+  All1 (noccurs x) ms -> n_ren ξ x ->
+  All1 (noccurs x) ms..[ren ξ].
+Proof.
+  move=>no. elim: no ξ=>//={ms}.
+  move=>ξ n. constructor.
+  move=> m ms nM nMs ih ξ n.
+  constructor.
+  apply: noccurs_ren; eauto.
+  apply: ih; eauto.
+Qed.
+
+Lemma pos_ren x A ξ :
+  pos x A -> n_ren ξ x -> pos x A.[ren ξ].
+Proof.
+  move=> p. elim: p ξ=>{x A}//=.
+  move=>x ms nms ξ [e h].
+  rewrite spine_subst=>//=.
+  rewrite e. constructor. by apply: noccurs_ren_All1.
+  move=>x A B s r t nA pB ihB ξ n.
+  constructor.
+  by apply: noccurs_ren.
+  asimpl. apply: ihB. by apply: n_ren_up.
+Qed.
+
+Lemma constr_ren i s C ξ :
+  constr i s C -> n_ren ξ i -> constr i s C.[ren ξ].
+Proof.
+  move=>c. elim: c ξ=>{i s C}.
+  move=>x s ms no ξ [e h].
+  { rewrite spine_subst. asimpl.
+    rewrite e.
+    constructor.
+    elim: no=>//=. constructor.
+    move=>m ls nm nms ih.
+    constructor.
+    apply: noccurs_ren; eauto; constructor; eauto.
+    apply: ih. }
+  move=>s t x A B leq pA nB cB ihB ξ n=>//=.
+  { apply: constr_pos; eauto.
+    apply: pos_ren; eauto.
+    asimpl. apply: noccurs_ren; eauto. apply: n_ren0.
+    asimpl. apply: ihB. apply: n_ren_up; eauto. }
+  move=>s t x A B leq nA cB ihB ξ n=>//=.
+  { apply: constr_pi; eauto.
+    apply: noccurs_ren; eauto.
+    asimpl. apply: ihB. apply: n_ren_up; eauto. }
+Qed.
+
+Lemma respine_respine0 k s s' c I :
+  (forall Q, respine k s Q c I = (s', kapp k Q c)) ->
+  (forall Q, respine0 Q I = Q).
+Proof.
+  elim: I=>//=.
+  move=>m _ n _ h Q.
+  destruct k.
+  have{}[e1 e2]//:=h Q.
+  have{}[e1 e2]//:=h Q.
+Qed.
+
+Lemma respine_ren1 k s s' (I : var -> term) :
+  (forall i c Q, respine k s Q c (I i) = (s', kapp k Q c)) ->
+  (forall i c Q, respine k s Q c (I i).[ren (+1)] = (s', kapp k Q c)).
+Proof.
+  move=>h i. move e:(I i)=>n.
+  elim: n e h=>//=.
+  move=>x e h c Q.
+  { erewrite<-(h i)=>//.
+    by rewrite e. }
+  move=>s0 l e h c Q.
+  { erewrite<-(h i)=>//.
+    by rewrite e. }
+  move=>A _ B _ s0 r t e h c Q.
+  { have:=h i c (Var 0).
+    rewrite e=>//=.
+    destruct k=>//=.
+    destruct (respine U s (ids 1) (App c.[ren (+1)] (Var 0)) B)=>//.
+    destruct (respine L s (ids 1) (App c.[ren (+1)] (Var 0)) B)=>//. }
+  move=>A _ m _ s0 t e h c Q.
+  { have:=h i c (Var 0).
+    rewrite e=>//=.
+    destruct k=>//=.
+    move=>[]->//.
+    move=>[]->//. }
+  move=>m _ n _ e h c Q.
+  { have:=h i c (Var 0).
+    rewrite e=>//=.
+    destruct k=>//=. }
+  move=>A _ Cs s0 e h c Q.
+  { have:=h i c (Var 0).
+    rewrite e=>//=.
+    destruct k=>//=.
+    move=>[]->//.
+    move=>[]->//. }
+  move=>i0 m _ e h c Q.
+  { have:=h i c (Var 0).
+    rewrite e=>//=.
+    destruct k=>//=.
+    move=>[]->//.
+    move=>[]->//. }
+  move=>m _ Q _ Fs e h c Q0.
+  { have:=h i c (Var 0).
+    rewrite e=>//=.
+    destruct k=>//=.
+    move=>[]->//.
+    move=>[]->//. }
+  move=>A _ m _ e h c Q.
+  { have:=h i c (Var 0).
+    rewrite e=>//=.
+    destruct k=>//=.
+    move=>[]->//.
+    move=>[]->//. }
+Qed.
+
+Lemma respine_up k s I :
+  (forall i c Q, respine k s Q c (I i) = (s, kapp k Q c)) ->
+  (forall i c Q, respine k s Q c (up I i) = (s, kapp k Q c)).
+Proof.
+  move=>h i. elim: i I h=>//=.
+  move=>I h c Q. destruct k=>//=.
+  move=>n ih I h c Q. asimpl.
+  by apply: respine_ren1.
+Qed.
+
+Lemma rearity_ren k s s' I A ξ :
+  arity s A -> (rearity k s' I A).[ren ξ] = rearity k s' I.[ren ξ] A.[ren ξ].
+Proof.
+  move=>ar. elim: ar I ξ s'=>{A}//=.
+  move=>l I ξ s'. destruct k=>//.
+  move=>A B ar ih I ξ s'. asimpl.
+  rewrite ih. by asimpl.
+Qed.
+
+Lemma respine0_I_ren Q I ξ :
+  (forall Q, respine0 Q I = Q) -> Q.[ren ξ] = respine0 Q.[ren ξ] I.[ren ξ].
+Proof.
+  elim: I ξ Q=>//=.
+  move=>m _ n _ ξ Q h.
+  have//=:=h (Var 0).
+Qed.
+
+Lemma respine_I_ren k s s' Q c I ξ :
+  (forall c Q, respine k s Q c I = (s', kapp k Q c)) ->
+  s' = (respine k s Q.[ren ξ] c.[ren ξ] I.[ren ξ]).1 /\
+  kapp k Q.[ren ξ] c.[ren ξ] = (respine k s Q.[ren ξ] c.[ren ξ] I.[ren ξ]).2.
+Proof.
+  elim: I ξ c Q=>//=.
+  move=>x ξ c Q h.
+  { destruct k=>//=.
+    have[->]//:=h c Q.
+    have[->]//:=h c Q. }
+  move=>t i ξ c Q h.
+  { destruct k=>//=.
+    have[->]//:=h c Q.
+    have[->]//:=h c Q. }
+  move=>A _ B _ s0 r t ξ c Q h.
+  { have{h}:=h c (Var 0).
+    destruct k=>//=.
+    destruct (respine U s (ids 1) (App c.[ren (+1)] (Var 0)) B)=>//.
+    destruct (respine L s (ids 1) (App c.[ren (+1)] (Var 0)) B)=>//. }
+  move=>A _ m _ r t ξ c Q h.
+  { destruct k=>//=.
+    have[->]//:=h c Q.
+    have[->]//:=h c Q. }
+  move=>m _ n _ ξ c Q h.
+  { have{h}:=h c (Var 0).
+    destruct k=>//=. }
+  move=>A _ Cs r ξ c Q h.
+  { destruct k=>//=.
+    have[->]//:=h c Q.
+    have[->]//:=h c Q. }
+  move=>i m _ ξ c Q h.
+  { destruct k=>//=.
+    have[->]//:=h c Q.
+    have[->]//:=h c Q. }
+  move=>m _ Q _ Fs ξ c Q0 h.
+  { destruct k=>//=.
+    have[->]//:=h c Q.
+    have[->]//:=h c Q. }
+  move=>A _ m _ ξ c Q h.
+  { destruct k=>//=.
+    have[->]//:=h c Q.
+    have[->]//:=h c Q. }
+Qed.
+
+Lemma kapp_ren k m n ξ : (kapp k m n).[ren ξ] = kapp k m.[ren ξ] n.[ren ξ].
+Proof. destruct k=>//=. Qed.
+
+Lemma respine0_spine'_I_ren Q I ms ξ :
+  (forall Q, respine0 Q I = Q) ->
+  (respine0 Q (spine' I ms)).[ren ξ] = respine0 Q.[ren ξ] (spine' I ms).[ren ξ].
+Proof.
+  elim: ms Q ξ=>//=.
+  move=>Q ξ h. rewrite h. by apply: respine0_I_ren.
+  move=>a l ih Q ξ h.
+  rewrite ih=>//.
+Qed.
+
+Lemma respine_spine'_I_ren k s s' Q c I ms ξ :
+  (forall c Q, respine k s Q c I = (s', kapp k Q c)) ->
+  (respine k s Q c (spine' I ms)).1 =
+    (respine k s Q.[ren ξ] c.[ren ξ] (spine' I ms).[ren ξ]).1 /\
+  (respine k s Q c (spine' I ms)).2.[ren ξ] =
+    (respine k s Q.[ren ξ] c.[ren ξ] (spine' I ms).[ren ξ]).2.
+Proof.
+  elim: ms Q c ξ=>//=.
+  move=>Q c ξ h.
+  rewrite h=>//=.
+  rewrite kapp_ren.
+  by apply: respine_I_ren.
+  move=>a l ih Q c ξ h.
+  destruct k=>//=.
+  rewrite respine0_spine'_I_ren; eauto.
+  by apply: respine_respine0.
+  rewrite respine0_spine'_I_ren; eauto.
+  by apply: respine_respine0.
+  Unshelve. eauto. eauto.
+Qed.
+
+Lemma respine_spine_I_ren k s s' I :
+  (forall c Q, respine k s Q c I = (s', kapp k Q c)) ->
+  forall c Q ms ξ,
+    (respine k s Q c (spine I ms)).1 =
+      (respine k s Q.[ren ξ] c.[ren ξ] (spine I ms).[ren ξ]).1 /\
+    (respine k s Q c (spine I ms)).2.[ren ξ] =
+      (respine k s Q.[ren ξ] c.[ren ξ] (spine I ms).[ren ξ]).2.
+Proof.
+  move=>h c Q ms ξ.
+  rewrite spine_spine'_rev.
+  by apply: respine_spine'_I_ren.
+Qed.
+
+Lemma constr_respine_ren x s' C :
+  constr x s' C ->
+  forall k s I, (forall i c Q, respine k s Q c (I i) = (s, kapp k Q c)) ->
+  forall c Q ξ,
+    (respine k s Q c C.[I]).1 =
+      (respine k s Q.[ren ξ] c.[ren ξ] C.[I].[ren ξ]).1 /\
+    (respine k s Q c C.[I]).2.[ren ξ] =
+      (respine k s Q.[ren ξ] c.[ren ξ] C.[I].[ren ξ]).2.
+Proof.
+  move=>cn. elim: cn=>{x s' C}.
+  move=>x s' ms nms k s0 I h c Q ξ.
+  { rewrite!spine_subst. asimpl.
+    pose proof (respine_spine_I_ren (h x) c Q ms..[I] ξ) as X.
+    rewrite!spine_subst in X.
+    by asimpl in X. }
+  move=>s t x A B leq pA nB cB ih k s0 I h c Q ξ.
+  { asimpl.
+    have/ih{}ih:=respine_up h.
+    pose proof (ih (App c.[ren (+1)] (Var 0)) Q.[ren (+1)] (upren ξ)) as hx.
+    asimpl in hx.
+    replace (Var 0) with (ids 0) in hx by autosubst.
+    replace (Var 0) with (ids 0) by autosubst.
+    remember (respine k s0 Q.[ren (+1)] (App c.[ren (+1)] (ids 0)) B.[up I]) as p1.
+    remember (respine k s0 Q.[ren (ξ >>> (+1))] (App c.[ren (ξ >>> (+1))] (ids 0))
+       B.[ids 0 .: I >> ren (ξ >>> (+1))]) as p2.
+    destruct p1. destruct p2.
+    split; eauto.
+    asimpl. simpl in hx. destruct hx.
+    repeat f_equal; eauto. }
+  move=>s t x A B leq nA cB ih k s0 I h c Q ξ.
+  { asimpl.
+    have/ih{}ih:=respine_up h.
+    pose proof (ih (App c.[ren (+1)] (Var 0)) Q.[ren (+1)] (upren ξ)) as hx.
+    asimpl in hx.
+    replace (Var 0) with (ids 0) in hx by autosubst.
+    replace (Var 0) with (ids 0) by autosubst.
+    remember (respine k s0 Q.[ren (+1)] (App c.[ren (+1)] (ids 0)) B.[up I]) as p1.
+    remember (respine k s0 Q.[ren (ξ >>> (+1))] (App c.[ren (ξ >>> (+1))] (ids 0))
+       B.[ids 0 .: I >> ren (ξ >>> (+1))]) as p2.
+    destruct p1. destruct p2.
+    split; eauto.
+    asimpl. simpl in hx. destruct hx.
+    repeat f_equal; eauto. }
+Qed.
+
+Lemma All2_case_ren Γ Γ' n k s s' A Q Fs Cs Cs' ξ :
+  All2i (fun i F C =>
+    constr 0 s C /\
+    let I := Ind A Cs' s in
+    let T := mkcase k s' I Q (Constr i I) C in
+    forall Γ' ξ, agree_ren ξ Γ Γ' ->
+      Γ' ⊢ F.[ren ξ] : T.2.[ren ξ] : T.1) n Fs Cs ->
+  agree_ren ξ Γ Γ' ->
+  All2i (fun i F C =>
+    constr 0 s C /\
+    let I := Ind A.[ren ξ] Cs'..[up (ren ξ)] s in
+    let T := mkcase k s' I Q.[ren ξ] (Constr i I) C in
+    Γ' ⊢ F : T.2 : T.1) n Fs..[ren ξ] Cs..[up (ren ξ)].
+Proof.
+  elim: Fs Γ Γ' n s A Q Cs ξ=>//=.
+  move=>Γ Γ' n s A Q Cs ξ h agr. inv h.
+  { constructor. }
+  move=>F Fs ih Γ Γ' n s A Q Cs ξ h agr.
+  inv h. inv H2.
+  constructor.
+  { split.
+    asimpl.
+    apply: constr_ren; eauto. apply: n_ren0.
+    have{H0}tyF:=H0 _ _ agr.
+    unfold mkcase in tyF.
+    have h: ∀ i c Q, respine k s' Q c ((Ind A Cs' s .: ids) i) = (s', kapp k Q c).
+    { move=>[|i] c Q0; asimpl.
+      destruct k=>//.
+      destruct k=>//. }
+    have {h}[e1 e2]:=constr_respine_ren H h (Constr n (Ind A Cs' s)) Q ξ.
+    rewrite e1 in tyF=>{e1}.
+    rewrite e2 in tyF=>{e2}.
+    asimpl in tyF.
+    unfold mkcase.
+    asimpl. eauto. }
+  { apply: ih; eauto. }
+Qed.
+
 Lemma rename_ok Γ Γ' m A s ξ :
   Γ ⊢ m : A : s -> agree_ren ξ Γ Γ' -> Γ' ⊢ m.[ren ξ] : A.[ren ξ] : s.
 Proof with eauto using 
   clc_type, agree_ren, agree_ren_key, agree_ren_re_re.
-  move=>ty. elim: ty Γ' ξ=>{Γ m A s}.
+  move=>ty. move: Γ m A s ty Γ' ξ.
+  apply: clc_type_ind_nested=>//=.
   move=>Γ s l k Γ' ξ agr. asimpl...
   move=>Γ A B [] r t i k tyA ihA tyB ihB Γ' ξ agr.
   { asimpl.
@@ -144,72 +520,46 @@ Proof with eauto using
       by autosubst.
     apply: clc_app...
     asimpl in tym... }
-  move=>Γ k Γ' ξ arg. asimpl...
-  move=>Γ k Γ' ξ arg. asimpl...
-  move=>Γ k Γ' ξ agr. asimpl...
-  move=>Γ k Γ' ξ agr. asimpl...
-  move=>Γ k Γ' ξ agr. asimpl...
-  move=>Γ A B s r t i leq k tyA ihA tyB ihB Γ' ξ agr.
+  move=>Γ A Cs s t l k ar ctr tyA ihA tyCs ihCs Γ' ξ agr.
   { asimpl.
-    destruct s.
-    have:agree_ren (upren ξ) (A :U [Γ]) (A.[ren ξ] :U [Γ'])...
-    have:agree_ren (upren ξ) (_: [Γ]) (_: [Γ'])... }
-  move=>Γ1 Γ2 Γ A B m n s r t i k1 k2 mrg 
-    tyS ihS tym ihm tyn ihn Γ' ξ agr.
-  { asimpl.
-    move:(merge_agree_ren_inv agr mrg)=>[G1[G2[mrg1[agr1 agr2]]]].
-    move:(agree_ren_key agr1 k1)=>{}k1.
-    move:(agree_ren_key agr2 k2)=>{}k2.
-    apply: clc_pair...
-    move:(ihS _ _ (agree_ren_re_re agr)). asimpl...
-    move:(ihn _ _ agr2). asimpl... }
-  move=>Γ1 Γ2 Γ m n1 n2 A s t i k mrg tym ihm tyA ihA tyn1 ihn1 tyn2 ihn2 Γ' ξ agr.
-  { asimpl.
+    apply: clc_indd...
+    apply: arity_ren...
+    move=>{agr}.
+    elim: ctr ξ=>//=...
+    { move=>_. constructor. }
+    { move=>m ls c h ih ξ. asimpl.
+      constructor.
+      apply: constr_ren... apply: n_ren0.
+      have:=ih ξ... }
+    elim: ihCs=>//=.
+    { constructor. }
+    { move=>m ls ihm hls ihls. asimpl.
+      constructor... } }
+  move=>Γ A s i C Cs k ig ty ih Γ' ξ agr.
+  { replace (C.[Ind A Cs s/].[ren ξ])
+      with (C.[up (ren ξ)]).[Ind A.[ren ξ] Cs..[up (ren ξ)] s/]
+        by autosubst.
+    apply: clc_constr...
+    apply: iget_subst... }
+  move=>Γ1 Γ2 Γ A Q s s' k Fs Cs m ms leq ar mrg tym ihm tyQ ihQ tyFs ihFs Γ' ξ agr.
+  { rewrite kapp_ren.
+    rewrite spine_subst.
     have[G1[G2[mrg'[agr1 agr2]]]]:=merge_agree_ren_inv agr mrg.
-    have//={}ihm:=ihm _ _ agr1.
-    have//={}ihn1:=ihn1 _ _ agr2. asimpl in ihn1.
-    have//={}ihn2:=ihn2 _ _ agr2. asimpl in ihn2.
-    replace A.[m.[ren ξ] .: ren ξ] with A.[up (ren ξ)].[m.[ren ξ]/] by autosubst.
-    have/ihA{}ihA:agree_ren (upren ξ) [Either :{s} Γ2] [Either :{s} G2].
-    { destruct s; simpl; constructor... }
-    asimpl in ihA.
-    have{}k:=agree_ren_key agr1 k.
-    apply: clc_case...
-    asimpl...
-    asimpl...
-    asimpl... }
-  move=>Γ1 Γ2 Γ m n A s mrg tym ihm tyn ihn Γ' ξ agr.
+    have ar':=arity_ren ξ ar.
+    have{}ihm:=ihm _ _ agr1. rewrite spine_subst in ihm.
+    have{}ihQ:=ihQ _ _ (agree_ren_re_re agr2).
+    rewrite (rearity_ren k s' (Ind A Cs s) ξ ar) in ihQ.
+    apply: clc_case; eauto.
+    apply: All2_case_ren; eauto. }
+  move=>Γ A m l k tyA ihA tym ihm Γ' ξ agr.
   { asimpl.
-    move:(merge_agree_ren_inv agr mrg)=>[G1[G2[mrg1[agr1 agr2]]]].
-    move:(ihm _ _ agr1)=>{}ihm.
-    move:(ihn _ _ agr2)=>{}ihn.
-    apply: clc_letin1... }
-  move=>Γ1 Γ2 Γ A B C m n s r t k x i leq key mrg 
-    tym ihm tyC ihC tyn ihn Γ' ξ agr.
-  { asimpl.
-    move:(merge_agree_ren_inv agr mrg)=>[G1[G2[mrg1[agr1 agr2]]]].
-    move:(ihm _ _ agr1)=>{ihm}tym.
-    move:(agree_ren_key agr1 key)=>{}key.
-    have/ihn{ihn}tyn:agree_ren (upren (upren ξ)) (B :{r} A :{s} Γ2)
-      (B.[ren (upren ξ)] :{r} A.[ren ξ] :{s} G2)...
-    destruct k.
-    have/ihC{ihC}tyC:agree_ren (upren ξ) (Sigma A B s r t :U [Γ2])
-      ((Sigma A B s r t).[ren ξ] :U [G2])...
-    asimpl in tym.
-    asimpl in tyC.
-    replace C.[Pair (Var 1) (Var 0) t .: ren (+2)].[ren (upren (upren ξ))]
-      with C.[ren (upren ξ)].[Pair (Var 1) (Var 0) t .: ren (+2)]
-        in tyn by autosubst.
-    have:=clc_letin2 leq key mrg1 tym tyC tyn.
-    by asimpl.
-    have/ihC{ihC}tyC:agree_ren (upren ξ) (_: [Γ2]) (_: [G2])...
-    asimpl in tym.
-    asimpl in tyC.
-    replace C.[Pair (Var 1) (Var 0) t .: ren (+2)].[ren (upren (upren ξ))]
-      with C.[ren (upren ξ)].[Pair (Var 1) (Var 0) t .: ren (+2)]
-        in tyn by autosubst.
-    have:=clc_letin2 leq key mrg1 tym tyC tyn.
-    by asimpl. }
+    apply: clc_fix.
+    apply: agree_ren_key; eauto.
+    apply: ihA; eauto.
+    replace A.[ren ξ].[ren (+1)] with A.[ren (+1)].[ren (upren ξ)]
+      by autosubst.
+    apply: ihm.
+    by constructor. }
   move=>Γ A B m s i sb tym ihm tyB ihB Γ' ξ agr.
   { move:(ihm _ _ agr)=>{ihm}tym.
     move:(ihB _ _ (agree_ren_re_re agr))=>{ihB}tyB.
