coq/cilc2/clc_subtype.v
@@ -14,11 +14,7 @@ Inductive sub1 : term -> term -> Prop :=
   sub1 (s @ l1) (s @ l2)
 | sub1_pi A B1 B2 s r t : 
   sub1 B1 B2 -> 
-  sub1 (Pi A B1 s r t) (Pi A B2 s r t)
-| sub1_sigma A1 A2 B1 B2 s r t :
-  sub1 A1 A2 ->
-  sub1 B1 B2 ->
-  sub1 (Sigma A1 B1 s r t) (Sigma A2 B2 s r t).
+  sub1 (Pi A B1 s r t) (Pi A B2 s r t).
 
 CoInductive sub (A B : term) : Prop :=
 | SubI A' B' : 
@@ -45,8 +41,7 @@ Proof with eauto 6 using sub1, sub1_sub, sub1_conv, conv_sub1.
   move=> sb. elim: sb C D => {A B}
     [ A C D 
     | s l1 l2 leq C D conv sb
-    | A B1 B2 s r t sb1 ih C D conv sb2 
-    | A1 A2 B1 B2 s r t sb1 ih1 sb2 ih2 C D conv sb3 ]...
+    | A B1 B2 s r t sb1 ih C D conv sb2]...
   inv sb; try (exfalso; solve_conv)...
     move: conv => /sort_inj [->eq].
     apply: sub_sort. subst.
@@ -58,16 +53,6 @@ Proof with eauto 6 using sub1, sub1_sub, sub1_conv, conv_sub1.
     apply sub1_pi with (s := s0) (r := r0) (t := t0)... 
     exact: conv_pi. 
     exact: conv_pi.
-  inv sb3; try (exfalso; solve_conv)...
-    move: conv => /sigma_inj[conv1[conv2[->[->->]]]].
-    move: (ih1 _ _ conv1 H)=>{ih1}sub1.
-    move: (ih2 _ _ conv2 H0)=>{ih2}sub2.
-    inv sub1. inv sub2.
-    apply: SubI.
-    apply sub1_sigma with (s := s0) (r := r0) (t := t0).
-    exact: H1. exact: H4.
-    exact: conv_sigma.
-    exact: conv_sigma.
 Qed.
 
 Lemma sub_trans B A C :
@@ -88,7 +73,28 @@ Proof.
     inv l=> //.
   move=> s l0 l3 leq /sort_inj[->->]/sort_inj[<-<-]=> //.
   move=> *. exfalso; solve_conv.
-  move=> *. exfalso; solve_conv.
+Qed.
+
+Lemma sub_sort_false1 l1 l2 : ~U @ l1 <: L @ l2.
+Proof.
+  move=>[s1 s2[]].
+  move=>A e1 e2.
+    have e : U @ l1 === L @ l2.
+      exact: conv_trans e2.
+    solve_conv.
+  move=>s l3 l4 _/sort_inj[<-_]h. solve_conv.
+  move=>A B1 B2 s r t _ e1 e2. solve_conv.
+Qed.
+
+Lemma sub_sort_false2 l1 l2 : ~L @ l1 <: U @ l2.
+Proof.
+  move=>[s1 s2[]].
+  move=>A e1 e2.
+    have e : L @ l1 === U @ l2.
+      exact: conv_trans e2.
+    solve_conv.
+  move=>s l3 l4 _/sort_inj[<-_]h. solve_conv.
+  move=>A B1 B2 s r t _ e1 e2. solve_conv.
 Qed.
 
 Lemma sub_pi_inv A1 A2 s1 s2 r1 r2 t1 t2 B1 B2 :
@@ -106,24 +112,6 @@ Proof.
     /pi_inj[c1[c2[<-[<-<-]]]]/pi_inj[c3[c4[->[->->]]]]. 
     firstorder.
     exact: conv_trans c3. exact: SubI sb c2 c4.
-  move=> *. exfalso; solve_conv.
-Qed.
-
-Lemma sub_sigma_inv A1 A2 B1 B2 p1 p2 q1 q2 s1 s2 :
-  Sigma A1 B1 p1 q1 s1 <: Sigma A2 B2 p2 q2 s2 -> 
-  A1 <: A2 /\ B1 <: B2 /\ p1 = p2 /\ q1 = q2 /\ s1 = s2.
-Proof.
-  move=> [A' B' []].
-  move=> C c1 c2. 
-    have{c1 c2}/sigma_inj[c1[c2[->[->->]]]]: 
-      Sigma A1 B1 p1 q1 s1 === Sigma A2 B2 p2 q2 s2.
-    exact: conv_trans c2.
-    firstorder=>//. exact: conv_sub. exact: conv_sub.
-  move=> *. exfalso; solve_conv.
-  move=> *. exfalso; solve_conv.
-  move=>A A0 B0 B3 s r t sb1 sb2
-    /sigma_inj[c1[c2[<-[<-<-]]]]/sigma_inj[c3 [c4 [->[->->]]]]. 
-    firstorder. exact: SubI sb1 c1 c3. exact: SubI sb2 c2 c4.
 Qed.
 
 Lemma sub1_subst σ A B : sub1 A B -> sub1 A.[σ] B.[σ].
@@ -134,3 +122,22 @@ Proof. move=> [A' B' /sub1_subst]; eauto using sub, conv_subst. Qed.
 
 Lemma sub_ren A B ξ : A <: B -> A.[ren ξ] <: B.[ren ξ].
 Proof. move=> *; by apply: sub_subst. Qed.
+
+Ltac solve_sub :=
+  match goal with
+  | [ H : _ <: _ |- _ ] =>
+    let A := fresh "A" in
+    let B := fresh "B" in
+    let sb := fresh "sb" in
+    let c1 := fresh "c1" in
+    let c2 := fresh "c2" in
+    destruct H as [A B sb c1 c2]; destruct sb
+  end;
+  match goal with
+  | [ c1 : ?A === ?x, c2 : ?x === ?B |- _ ] =>
+    assert (A === B) by
+      (eapply conv_trans; try solve [apply c1| apply c2]);
+    clear c1 c2;
+    solve_conv
+  | _ => solve_conv
+  end.
